Improved the semantic AST. Extended stm command so that it generates a dataspace. Integrated the Circus RoboChart state machine semantics.

RoboChart/RoboChart_StateMachine.thy
@@ -4,13 +4,15 @@ theory RoboChart_StateMachine
   imports "RoboChart_AST"
 begin
 
+subsection \<open> Semantic AST \<close>
+
 text \<open> The following types represent state machines that have been supplied with typed contextual
   information. Predicates, actions, and expressions have all been enriched with type data, which
   is carried using the type parameters. \<close>
 
 datatype ('pred, 'act, 'prob) STransition = 
   STransition (tn_source: ID) (tn_target: ID) (tn_trigger: "'act option")
-              (tn_probability: "'prob option") (tn_condition: "'pred option") (tn_action: "'act option")
+              (tn_probability: "'prob option") (tn_cond: "'pred option") (tn_act: "'act option")
 
 datatype ('pred, 'act, 'prob) SNode =
   SNode (n_name: ID) (n_entry: "'act option") (n_during: "'act option") (n_exit: "'act option") 
@@ -21,17 +23,100 @@ datatype ('pred, 'act, 'prob) SStateMachine =
                 (sm_nodes: "('pred, 'act, 'prob) SNode list")
                 (sm_transitions: "('pred, 'act, 'prob) STransition list")
 
-(*
-notation sm_initial ("init\<index>")
-notation sm_finals ("finals\<index>")
-notation sm_nodes ("nodes\<index>")
+notation sm_initial ("Init\<index>")
+notation sm_finals ("Finals\<index>")
+notation sm_nodes ("Nodes\<index>")
 notation sm_transitions ("\<^bold>T\<index>")
-*)
 
-definition "mk_None = const @{const_name None}"
-definition "mk_Some t = const @{const_name Some} $ t"
-fun mk_option :: "term option \<Rightarrow> term" where
-"mk_option (Some t) = mk_Some t" | "mk_option None = mk_None"
+subsection \<open> Query Functions \<close>
+
+definition sm_node_names :: "('pred, 'act, 'prob) SStateMachine \<Rightarrow> String.literal set" ("Nnames\<index>") where
+"sm_node_names sm \<equiv> n_name ` set(sm_nodes sm)"
+
+definition sm_inters :: "('pred, 'act, 'prob) SStateMachine \<Rightarrow> ('pred, 'act, 'prob) SNode list" where
+"sm_inters sm = filter (\<lambda> n. n_name n \<notin> set(sm_finals sm)) (sm_nodes sm)"
+
+definition sm_inter_names ("Inames\<index>") where
+"sm_inter_names sm \<equiv> n_name ` set (sm_inters sm)"
+
+abbreviation sm_final_names ("Fnames\<index>") where
+"sm_final_names M \<equiv> set (Finals\<^bsub>M\<^esub>)"
+
+definition sm_node_map :: 
+  "('pred, 'act, 'prob) SStateMachine \<Rightarrow> (ID \<rightharpoonup> ('pred, 'act, 'prob) SNode)" ("Nmap\<index>") where
+"sm_node_map M = map_of (map (\<lambda> n. (n_name n, n)) (sm_nodes M))"
+
+definition sm_trans_map :: 
+  "('pred, 'act, 'prob) SStateMachine \<Rightarrow> (ID \<rightharpoonup> ('pred, 'act, 'prob) STransition list)" ("Tmap\<index>") where
+"sm_trans_map M = map_of (map (\<lambda> n. (n_name n, filter (\<lambda> t. tn_source t = n_name n) (sm_transitions M))) (sm_nodes M))"
+
+lemma dom_sm_node_map: "dom(Nmap\<^bsub>M\<^esub>) = Nnames\<^bsub>M\<^esub>"
+  using image_iff by (force simp add: sm_node_map_def sm_node_names_def dom_map_of_conv_image_fst)
+
+lemma dom_sm_trans_map: "dom(Tmap\<^bsub>M\<^esub>) = Nnames\<^bsub>M\<^esub>"
+  using image_iff by (force simp add: sm_trans_map_def sm_node_names_def dom_map_of_conv_image_fst)
+
+lemma nnames_finite: "finite(Nnames\<^bsub>M\<^esub>)"
+  by (force simp add: sm_node_names_def)
+
+abbreviation sm_init_node :: 
+  "('pred, 'act, 'prob) SStateMachine \<Rightarrow> ('pred, 'act, 'prob) SNode" ("Ninit\<index>") where
+"sm_init_node M \<equiv> the (sm_node_map M (sm_initial M))"
+
+subsection \<open> Well-formedness \<close>
+
+locale WfStateMachine =
+  fixes M :: "('pred, 'act, 'prob) SStateMachine" (structure)
+  \<comment> \<open> The list of nnames is a set \<close>
+  assumes nnames_distinct: "distinct (map n_name Nodes)"
+  and init_is_state: "Init \<in> Nnames"
+  and init_not_final: "Init \<notin> Fnames"
+  and trans_wf: " \<And> t. t \<in> set(\<^bold>T) \<Longrightarrow> tn_source t \<in> Inames \<and> tn_target t \<in> Nnames"
+begin
+  lemma init_is_inter: "Init \<in> Inames"
+    using init_is_state init_not_final by (auto simp add: sm_inters_def sm_inter_names_def sm_node_names_def)
+
+  lemma nmap_init: "Nmap Init = Some Ninit"
+    by (metis domIff dom_sm_node_map init_is_state option.exhaust_sel)
+
+  lemma n_name_init: "n_name Ninit = Init"
+  proof (simp add: sm_node_map_def)
+    have "map_of (map (\<lambda>n. (n_name n, n)) Nodes) Init = Some (the (map_of (map (\<lambda>n. (n_name n, n)) Nodes) Init))"
+      by (metis (no_types) nmap_init sm_node_map_def)
+    then show "n_name (the (map_of (map (\<lambda>n. (n_name n, n)) Nodes) Init)) = Init"
+      using map_of_SomeD by force
+  qed
+
+  lemma nmap_name:
+    assumes "n \<in> set Nodes"
+    shows "Nmap (n_name n) = Some n"
+  proof -
+    have "distinct (map fst (map (\<lambda>n. (n_name n, n)) Nodes))"
+      by (simp add: comp_def nnames_distinct)
+    with assms show ?thesis
+      by (simp add: sm_node_map_def)
+  qed
+
+  lemma ninit_is_node: "Ninit \<in> set Nodes"
+    using init_is_state nmap_name by (auto simp add: sm_node_names_def)
+
+  lemma tmap_node_in_trans: 
+    assumes "n \<in> Nnames" "ts \<in> ran(Tmap)"
+    shows "set(ts) \<subseteq> set(\<^bold>T)"
+    using assms by (auto simp add: sm_trans_map_def ran_distinct nnames_distinct comp_def)
+
+  lemma node_tran_exists:
+    assumes "n \<in> Nnames" "t \<in> set(the(Tmap n))"
+    shows "t \<in> set(\<^bold>T)"
+    by (metis (mono_tags, hide_lams) assms(1) assms(2) domIff dom_sm_trans_map in_mono init_is_state option.collapse ranI tmap_node_in_trans)
+
+end
+
+method check_machine uses defs = 
+  (unfold_locales, 
+   simp_all add: defs sm_node_names_def sm_inter_names_def sm_inters_def, safe, simp_all)
+
+subsection \<open> Compilation of Semantic State Machines \<close>
 
 abbreviation "read_opt_term ctx u \<equiv> mk_option (map_option (read_term ctx) u)"
 
