RoboChart/Semantics/Circus_Semantics/Circus_SM_Semantics.thy
@@ -1,0 +1,97 @@
+section \<open> Circus Statemachine Semantics \<close>
+
+theory Circus_SM_Semantics
+  imports "RoboChart.RoboChart" Actions
+begin
+
+subsection \<open> Alphabet \<close>
+
+alphabet robochart_ctrl =
+  rc_ctrl :: ID 
+
+type_synonym 's rcst = "'s robochart_ctrl_scheme"
+type_synonym ('s, 'e) RoboAction = "('s robochart_ctrl_scheme, 'e) Actions.Action"
+type_synonym 's RoboPred = "'s robochart_ctrl_scheme upred"
+
+translations
+  (type) "'s rcst" <= (type) "'s robochart_ctrl_scheme"
+  (type) "('s, 'e) RoboAction" <= (type) "('s rcst, 'e) Action"
+  (type) "'s RoboPred" <= (type) "'s rcst upred"
+
+abbreviation "rc_state \<equiv> robochart_ctrl.more\<^sub>L"
+
+notation rc_state ("\<^bold>r")
+
+syntax
+  "_svid_rc_state"  :: "svid" ("\<^bold>r")
+
+translations
+  "_svid_rc_state" == "CONST rc_state"
+  "_svid_dot \<^bold>r x" <= "x ;\<^sub>L \<^bold>r"
+
+type_synonym ('s, 'e) RTransition = "('s upred, ('s, 'e) Action, unit) STransition"
+type_synonym ('s, 'e) RNode = "('s upred, ('s, 'e) Action, unit) SNode"
+type_synonym ('s, 'e) RStateMachine = "('s upred, ('s, 'e) Action, unit) SStateMachine"
+
+subsection \<open> State Machine Semantics \<close>
+
+abbreviation "trigger_semantics t null_event \<equiv> 
+  (case tn_trigger t of 
+    Some e \<Rightarrow> if productive e then e else sync null_event | 
+    None \<Rightarrow> sync null_event)"
+
+definition tn_condition :: "('s, 'e) RTransition \<Rightarrow> 's upred" where
+"tn_condition t = case_option true_upred id (tn_cond t)"
+
+definition tn_action :: "('s, 'e) RTransition \<Rightarrow> ('s, 'e) Action" where
+"tn_action t = case_option skip id (tn_act t)"
+
+no_utp_lift tn_condition
+
+definition tr_semantics :: "('s, 'e) RTransition \<Rightarrow> (unit, 'e) chan \<Rightarrow> ('s, 'e) RoboAction" ("\<lbrakk>_\<rbrakk>\<^sub>T") where
+"tr_semantics t null_event \<equiv> 
+  tn_condition t \<oplus>\<^sub>p rc_state \<^bold>& 
+  rc_state:[trigger_semantics t null_event ; tn_action t]\<^sub>A\<^sup>+ ; rc_ctrl := \<guillemotleft>tn_target t\<guillemotright>"
+
+definition "n_entry_sem n = case_option skip id (n_entry n)"
+
+definition "n_exit_sem n = case_option skip id (n_exit n)"
+
+definition node_semantics :: 
+  "('s, 'e) RStateMachine \<Rightarrow> (unit, 'e) chan \<Rightarrow> ('s, 'e) RNode \<Rightarrow> ('s, 'e) RoboAction" ("_;_ \<turnstile> \<lbrakk>_\<rbrakk>\<^sub>N" [10,0,0] 10) where
+  "node_semantics M null_event node  = 
+  (rc_state:[n_entry_sem node]\<^sub>A\<^sup>+ ;
+   (foldr (\<box>) (map (\<lambda> t. \<lbrakk>t\<rbrakk>\<^sub>T null_event) (the (Tmap\<^bsub>M\<^esub> (n_name node)))) stop) ;
+   rc_state:[n_exit_sem node]\<^sub>A\<^sup>+)"
+
+definition sm_semantics :: "('s, 'e) RStateMachine \<Rightarrow> (unit, 'e) chan \<Rightarrow> ('s, 'e) RoboAction" ("\<lbrakk>_\<rbrakk>\<^sub>M") where
+"sm_semantics M null_event = 
+    (rc_ctrl := \<guillemotleft>sm_initial M\<guillemotright> ;
+    iteration (map (\<lambda> n. (&rc_ctrl =\<^sub>u \<guillemotleft>n_name n\<guillemotright>, M;null_event \<turnstile> \<lbrakk>n\<rbrakk>\<^sub>N)) (sm_inters M)))"
+
+lemmas sm_sem_def = sm_semantics_def node_semantics_def sm_inters_def sm_inter_names_def
+
+lemma tr_semantics_subst_ctrl: "[&rc_ctrl \<mapsto>\<^sub>s \<guillemotleft>k\<guillemotright>] \<dagger> (\<lbrakk>a\<rbrakk>\<^sub>T null_event) = \<lbrakk>a\<rbrakk>\<^sub>T null_event"
+  by (simp add: tr_semantics_def action_simp usubst unrest frame_asubst)
+
+lemma tr_choice_subst_ctrl:
+  "[&rc_ctrl \<mapsto>\<^sub>s \<guillemotleft>k\<guillemotright>] \<dagger> foldr (\<box>) (map (\<lambda>t. \<lbrakk>t\<rbrakk>\<^sub>T null_event) ts) stop = foldr (\<box>) (map (\<lambda>t. \<lbrakk>t\<rbrakk>\<^sub>T null_event) ts) stop"
+  by (induct ts, simp_all add: action_simp usubst tr_semantics_subst_ctrl)
+
+lemma sm_semantics_subst_ctrl:
+  "[&rc_ctrl \<mapsto>\<^sub>s \<guillemotleft>k\<guillemotright>] \<dagger> node_semantics M null_event node = node_semantics M null_event node"
+  by (simp add: node_semantics_def action_simp frame_asubst tr_choice_subst_ctrl unrest)
+
+stm stm1 =
+  var x :: int
+  initial s1
+  transition t1 [frm s1 to s2 condition "U(x = 0)" action "act(x := 1)"]
+
+context stm1
+begin
+
+thm machine_def
+
+end
+
+end
