RoboChart/Semantics/Circus_Semantics/ReactiveSpec.thy
@@ -1,0 +1,139 @@
+section \<open> Reactive Specifications \<close>
+
+theory ReactiveSpec
+  imports "UTP-Circus.utp_circus"
+begin
+
+consts
+  seq_comp :: "'a \<Rightarrow> 'a \<Rightarrow> 'a" (infixr ";" 61)
+
+typedef ('s, 'e) rrel = "{P :: ('s, 'e) action. (P is CDC) \<and> (P is CRR)}"
+  by (rule_tac x="false" in exI, simp add: closure)
+
+setup_lifting type_definition_rrel
+
+notation Rep_rrel ("\<lbrakk>_\<rbrakk>\<^sub>R")
+
+lemma rrel_eq_transfer: "P = Q \<longleftrightarrow> \<lbrakk>P\<rbrakk>\<^sub>R = \<lbrakk>Q\<rbrakk>\<^sub>R"
+  by (auto, metis Rep_rrel_inverse)
+
+instantiation rrel :: (type, type) refine
+begin
+  lift_definition less_eq_rrel :: "('a, 'b) rrel \<Rightarrow> ('a, 'b) rrel \<Rightarrow> bool" is "less_eq" .
+  lift_definition less_rrel :: "('a, 'b) rrel \<Rightarrow> ('a, 'b) rrel \<Rightarrow> bool" is "less" .
+instance by (intro_classes; transfer, simp add: less_uexpr_def)
+end
+
+lift_definition rconj :: "('s, 'e) rrel \<Rightarrow> ('s, 'e) rrel \<Rightarrow> ('s, 'e) rrel" is "(\<and>\<^sub>p)"
+  by (simp add: closure)
+
+adhoc_overloading uconj rconj
+
+lift_definition rdisj :: "('s, 'e) rrel \<Rightarrow> ('s, 'e) rrel \<Rightarrow> ('s, 'e) rrel" is "(\<or>\<^sub>p)"
+  by (simp add: closure)
+
+adhoc_overloading udisj rdisj
+
+(*
+lift_definition rnot :: "('s, 'e) rrel \<Rightarrow> ('s, 'e) rrel" is rea_not
+  by (simp add: closure)
+
+adhoc_overloading unot rnot
+
+definition rdiff :: "('s, 'e) rrel \<Rightarrow> ('s, 'e) rrel \<Rightarrow> ('s, 'e) rrel" where
+"rdiff P Q = (rconj P (rnot Q))"
+
+lift_definition rimplies :: "('s, 'e) rrel \<Rightarrow> ('s, 'e) rrel \<Rightarrow> ('s, 'e) rrel" is "op \<Rightarrow>\<^sub>r"
+  by (simp add: closure)
+
+adhoc_overloading uimpl rimplies
+*)
+
+lift_definition rfalse :: "('s, 'e) rrel" is false by (simp add: closure)
+
+adhoc_overloading ufalse rfalse
+
+lift_definition rtrue :: "('s, 'e) rrel" is true\<^sub>r by (simp add: closure)
+
+adhoc_overloading utrue rtrue
+
+(*
+interpretation boolean_algebra rdiff rnot rconj "op \<le>" "op <" rdisj rfalse rtrue
+  apply (unfold_locales)
+  apply (transfer, rel_auto)
+            apply (transfer, rel_auto)
+           apply (transfer, rel_auto)
+          apply (transfer, rel_auto)
+         apply (transfer, rel_auto)
+        apply (transfer, rel_auto)
+       apply (transfer, rel_auto)
+      apply (transfer)
+      apply (simp add: CRR_implies_RR truer_bottom_rpred)
+     apply (transfer)
+     apply (simp add: utp_pred_laws.sup_inf_distrib1)
+    apply (transfer, simp)
+  apply (transfer)
+   apply (simp add: CRR_implies_RR RR_implies_R1 rea_not_or)
+  apply (simp add: rdiff_def)
+  done
+*)
+
+lemma wp_rea_CRR_closed [closure]:
+  assumes "P is CRR" "Q is CRR"
+  shows "P wp\<^sub>r Q is CRR"
+  by (simp add: CRR_implies_RR rea_not_CRR_closed seq_CRR_closed wp_rea_def assms)
+
+lemma wp_rea_CDC_closed [closure]:
+  assumes "Q is CDC"
+  shows "P wp\<^sub>r Q is CDC"
+proof -
+  have "P wp\<^sub>r (CDC Q) is CDC"
+    by (rel_blast)
+  thus ?thesis
+    by (simp add: assms Healthy_if)
+qed
+
+lift_definition rwp ::
+  "('s, 'e) rrel \<Rightarrow> ('s, 'e) rrel \<Rightarrow> ('s, 'e) rrel" is "(wp\<^sub>r)"
+  by (simp add: closure)
+
+adhoc_overloading
+  uwp rwp
+
+lift_definition rseq :: 
+  "('s, 'e) rrel \<Rightarrow> ('s, 'e) rrel \<Rightarrow> ('s, 'e) rrel"  is "(;;)"
+  by (simp add: closure)
+
+adhoc_overloading
+  seq_comp rseq
+
+lift_definition rcondition :: "('s, 'e) rrel \<Rightarrow> bool" is "\<lambda> P. P is RC" .
+
+lemma rcondition_true: "rcondition true"
+  by (transfer, simp add: closure)
+
+lift_definition rsubst :: "'s usubst \<Rightarrow> ('s, 'e) rrel \<Rightarrow> ('s, 'e) rrel" is "st_subst"
+  by (simp add: closure)
+
+adhoc_overloading usubst rsubst
+
+lift_definition rR4 :: "('s, 'e) rrel \<Rightarrow> ('s, 'e) rrel" ("[_]\<^sub>\<rhd>") is "R4" by (simp add: closure)
+
+lift_definition rR5 :: "('s, 'e) rrel \<Rightarrow> ('s, 'e) rrel" ("[_]\<^sub>\<box>") is "R5" by (simp add: closure)
+
+lift_definition rcsp_do :: "'s upred \<Rightarrow> 's usubst \<Rightarrow> ('e list, 's) uexpr \<Rightarrow> ('s, 'e) rrel" ("\<^bold>\<Phi>'(_,_,_')") is csp_do
+  by (simp add: closure)
+
+lift_definition rcsp_enable :: "'s upred \<Rightarrow> ('e list, 's) uexpr \<Rightarrow> ('e set, 's) uexpr \<Rightarrow> ('s, 'e) rrel" ("\<^bold>\<E>'(_,_,_')") is csp_enable
+  by (simp add: closure)
+
+lift_definition runrest :: "('a \<Longrightarrow> ('s,'e) sfrd \<times> ('s,'e) sfrd) \<Rightarrow> ('s, 'e) rrel \<Rightarrow> bool" is "unrest_uexpr" .
+
+adhoc_overloading unrest runrest
+
+lemmas rrel_rep_eq = rtrue.rep_eq rfalse.rep_eq rconj.rep_eq rdisj.rep_eq rcsp_do.rep_eq rcsp_enable.rep_eq rrel_eq_transfer
+
+lemma rfalse_right_anhil [simp]: "P ; rfalse = rfalse"
+  by (transfer, simp)
+
+end
